working through notation changes

VCV-io/OracleComp/OracleComp.lean
@@ -5,7 +5,123 @@ Authors: Devon Tuma
 -/
 import «VCV-io».OracleComp.OracleSpec
 
+open OracleSpec
+
 inductive OracleComp (spec : OracleSpec) : Type → Type 1
   | pure' (α : Type) (a : α) : OracleComp spec α
   | query_bind' (i : spec.ι) (t : spec.domain i) (α : Type)
       (oa : spec.range i → OracleComp spec α) : OracleComp spec α
+
+namespace OracleComp
+
+variable {spec : OracleSpec} {α β γ : Type}
+
+def default_result : {α : Type} → OracleComp spec α → α
+  | _, pure' α a => a
+  | _, query_bind' _ _ α oa => default_result (oa default)
+
+instance (spec : OracleSpec) (α : Type) [h : Nonempty α] :
+  Nonempty (OracleComp spec α) := h.elim (λ x ↦ ⟨pure' α x⟩)
+
+instance (spec : OracleSpec) (α : Type) [Inhabited α] :
+  Inhabited (OracleComp spec α) := ⟨pure' α default⟩
+
+instance (spec : OracleSpec) (α : Type) [h : IsEmpty α] :
+  IsEmpty (OracleComp spec α) := ⟨λ oa ↦ h.1 (default_result oa)⟩
+
+def base_inhabited (oa : OracleComp spec α) : Inhabited α := ⟨oa.default_result⟩
+
+section Monad
+
+/-- We define a monadic bind operation on `oracle_comp` by induction on the first computation.
+With this definition `oracle_comp` satisfies the monad laws (see `oracle_comp.is_lawful_monad`). -/
+def bind' : (α β : Type) → OracleComp spec α → (α → OracleComp spec β) → OracleComp spec β
+| _, _, pure' α a, ob => ob a
+| _, β, query_bind' i t α oa, ob => query_bind' i t β (λ u ↦ bind' α β (oa u) ob)
+
+instance (spec : OracleSpec) : Monad (OracleComp spec) :=
+{ pure := @pure' spec, bind := @bind' spec }
+
+protected lemma pure_def (spec : OracleSpec) {α : Type} (a : α) :
+  (pure a : OracleComp spec α) = pure' α a := rfl
+
+protected lemma bind_def {spec : OracleSpec} {α β : Type}
+  (oa : OracleComp spec α) (ob : α → OracleComp spec β) :
+  oa >>= ob = bind' α β oa ob := rfl
+
+instance (spec : OracleSpec) : LawfulMonad (OracleComp spec) :=
+LawfulMonad.mk' _
+  (λ oa ↦ by
+    induction' oa with α a i t α oa hoa
+    · rfl
+    · exact congr_arg (query_bind' i t α) (funext (λ u ↦ hoa u)))
+  (λ x ob ↦ rfl)
+  (λ oa ob oc ↦ by
+    induction' oa with α a i t α oa hoa
+    · rfl
+    · refine congr_arg (query_bind' i t _) <| funext (λ u ↦ hoa u ob))
+
+-- @[simp] protected lemma pure'_eq_return (spec) :
+--   (pure' α : α → oracle_comp spec α) = return := funext (λ a ↦ rfl)
+
+-- @[simp] protected lemma pure_eq_return (spec) :
+--   (pure : α → oracle_comp spec α) = return := funext (λ a, rfl)
+
+-- @[simp] protected lemma bind'_eq_bind (spec) :
+--   (bind' α β : oracle_comp spec α → (α → oracle_comp spec β) → oracle_comp spec β) = (>>=) := rfl
+
+-- protected lemma bind_return_comp_eq_map (oa : OracleComp spec α) (f : α → β) :
+--   oa >>= pure ∘ f = f <$> oa := rfl
+
+-- protected lemma map_eq_bind_return_comp (oa : oracle_comp spec α) (f : α → β) :
+--   f <$> oa = oa >>= return ∘ f := rfl
+
+-- protected lemma return_bind (a : α) (ob : α → oracle_comp spec β) :
+--   return a >>= ob = ob a := pure_bind a ob
+
+-- protected lemma bind_return (oa : oracle_comp spec α) : oa >>= return = oa := bind_pure oa
+
+-- @[simp] lemma bind_query_bind' (i : spec.ι) (t : spec.domain i)
+--   (oa : spec.range i → oracle_comp spec α) (ob : α → oracle_comp spec β) :
+--   (query_bind' i t α oa) >>= ob = query_bind' i t β (λ u, oa u >>= ob) := rfl
+
+-- @[simp] lemma map_map_eq_map_comp (oa : oracle_comp spec α) (f : α → β) (g : β → γ) :
+--   g <$> (f <$> oa) = (g ∘ f) <$> oa :=
+-- by simp [oracle_comp.map_eq_bind_return_comp, bind_assoc]
+
+-- lemma map_return (f : α → β) (a : α) : f <$> (return a : OracleComp spec α) = return (f a) := rfl
+
+protected lemma bind_congr {oa oa' : OracleComp spec α} {ob ob' : α → OracleComp spec β}
+  (h : oa = oa') (h' : ∀ x, ob x = ob' x) : oa >>= ob = oa' >>= ob' :=
+h ▸ (congr_arg (λ ob ↦ oa >>= ob) (funext h'))
+
+lemma ite_bind (p : Prop) [Decidable p] (oa oa' : OracleComp spec α)
+  (ob : α → OracleComp spec β) : ite p oa oa' >>= ob = ite p (oa >>= ob) (oa' >>= ob) :=
+by split_ifs <;> rfl
+
+-- lemma bind_seq (oa : OracleComp spec α) (og : OracleComp spec (α → β))
+--   (oc : β → OracleComp spec γ) : (og <*> oa) >>= oc = og >>= λ f ↦ oa >>= (oc ∘ f) :=
+-- by simp [seq_eq_bind_map, map_eq_bind_pure_comp, bind_assoc]
+
+end Monad
+
+section query
+
+/-- Shorthand for running a query and returning the value.
+Generally this should be preferred over using `query_bind'` directly. -/
+def query (i : spec.ι) (t : spec.domain i) : OracleComp spec (spec.range i) :=
+query_bind' i t (spec.range i) (pure' (spec.range i))
+
+lemma query_def (i : spec.ι) (t : spec.domain i) :
+  query i t = query_bind' i t (spec.range i) (pure' (spec.range i)) := rfl
+
+@[simp] lemma query_bind'_eq_query_bind (i : spec.ι)
+  (t : spec.domain i) (oa : spec.range i → OracleComp spec α) :
+  query_bind' i t α oa = query i t >>= oa := rfl
+
+@[reducible, inline] def coin : OracleComp coinSpec Bool :=
+query (spec := coinSpec) () ()
+
+end query
+
+end OracleComp
